testdata/ocifetch/modulefile.cue
@@ -1,0 +1,2 @@
+module: "foo.example@v0"
+language: version: "v0.13.0"
